code/Folding.ec
@@ -1,0 +1,28 @@
+require import AllCore List.
+
+lemma bound_range (n m : int) :
+  all (fun i => n <= i < m) (range n m).
+proof.
+  smt.
+qed.
+
+lemma foldr_range b (f : int -> bool -> bool) n m:
+    foldr f b (range n m) = foldr (fun i acc => n <= i < m /\ f i acc) b (range n m).
+proof.
+  have := bound_range n m.
+  elim (range n m).
+  - progress.
+  - progress.
+  have -> : (n <= x && x < m) = true by smt().
+  simplify.
+  rewrite H. apply H2.
+  done.
+qed.
+
+lemma foldr_id (b : 'b) (xs : 'a list):
+    foldr (fun i acc => acc) b xs = b.
+proof.
+   elim xs; progress.
+qed.
+ 
+
